Parity correct

Hoare2.v
@@ -21,7 +21,7 @@ Proof.
             apply hoare_asgn.
         SCase "pre-condition weakening".
             intros st [HT GuardTrue]. unfold assn_sub. apply HT.
-    Case "strenghening the post-condition".
+    Case "strengthening the post-condition".
         intros st [HT GuardFalse].
         unfold bassn in GuardFalse. simpl in GuardFalse.
         SearchAbout [not true].
@@ -31,6 +31,110 @@ Proof.
         SearchAbout [beq_nat true].
         apply beq_nat_true in GuardFalse.
         apply GuardFalse.
+Qed.
+
+(* slow_assignment:
+
+   loop invariant is X + Y = m
+
+    {{ X = m }}
+    Y ::= 0;
+    {{ X + Y = m }}
+    WHILE X <> 0 DO
+        {{ X + Y = m /\ X <> 0 }} ->>   (OK)
+        {{ (X - 1) + (Y + 1) = m }}
+        X ::= X - 1;
+        {{ X + (Y + 1) = m }}
+        Y ::= Y + 1;
+        {{ X + Y = m }}
+    END
+    {{ X + Y = m /\ ~(X <> 0) }} ->>    (OK)
+    {{ Y = m }}
+
+*)
+
+(* add_slowly_decoration:
+
+   loop invariant is X + Z = m + n
+
+{{ X = m /\ Z = n }} ->>                (OK)
+{{ X + Z = m + n }}
+WHILE X <> 0 DO
+    {{ X + Z = m + n /\ X <> 0 }} ->>   (OK)
+    {{ (X - 1) + (Z + 1) = m + n }}
+    Z ::= Z + 1;
+    {{ (X - 1) + Z = m + n }}
+    X ::= X - 1;
+    {{ X + Z = m + n }}
+END
+{{ X + Z = m + n /\ ~(X <> 0) }} ->>    (OK)
+{{ Z = n + m }}
+
+*)
+
+Fixpoint parity x :=
+    match x with
+    | 0 => 0
+    | 1 => 1
+    | S (S x') => parity x'
+    end.
+
+Lemma parity_ge_2: forall x,
+    2 <= x ->
+    parity (x - 2) = parity x.
+Proof.
+    induction x; intro.
+    Case "base". reflexivity.
+    Case "step". destruct x.
+        SCase "O". inversion H. inversion H1.
+        SCase "S ..". simpl. rewrite <- minus_n_O. reflexivity.
+Qed.
+
+Lemma parity_lt_2: forall x,
+    ~ ( 2 <= x ) ->
+    parity x = x.
+Proof.
+    induction x; intro.
+    Case "base". reflexivity.
+    Case "step". unfold not in H. destruct x.
+        SCase "O". reflexivity.
+        SCase "S ..". apply ex_falso_quodlibet. apply H. omega.
+Qed.
+
+Theorem parity_correct: forall m,
+    {{ fun st => st X = m }}
+    WHILE BLe (ANum 2) (AId X) DO
+        X ::= AMinus (AId X) (ANum 2)
+    END
+    {{ fun st => st X = parity m }}.
+Proof.
+    intro m.
+    (* we nee to adjust both the pre- and post-condition *)
+    eapply hoare_consequence.
+    Case "hoare_while".
+        (* loop with its invariant; crucial step *)
+        apply hoare_while
+            with (P := (fun st => parity (st X) = parity m)).
+        (* fix the inner part of the loop *)
+        eapply hoare_consequence_pre.
+        SCase "assignment".
+            apply hoare_asgn.
+        SCase "assignment pre-condition weakening".
+            unfold assert_implies, assn_sub, update. simpl.
+            intros st [H0 H1]. rewrite <- H0. apply parity_ge_2.
+            unfold bassn, beval, aeval in H1.
+            apply ble_nat_true in H1. apply H1.
+    Case "weakening the pre-condition".
+        unfold assert_implies. intros st H.
+        rewrite -> H. reflexivity.
+    Case "strengthening the post-condition".
+        unfold bassn, assert_implies. intros st [H0 H1].
+        rewrite <- H0. symmetry. apply parity_lt_2.
+        unfold beval, aeval in H1.
+        (* destruct and remember *)
+        destruct (ble_nat 2 (st X)) eqn:Heqle.
+        apply ex_falso_quodlibet. apply H1. reflexivity.
+        apply ble_nat_false in Heqle. apply Heqle.
 Qed.
 
 
